<?xml version="1.0"?>
<rdf:RDF xmlns="http://smartcities.linkeddata.es/airQuality/ontology#"
     xml:base="http://smartcities.linkeddata.es/airQuality/ontology"
     xmlns:om="http://www.ontology-of-units-of-measure.org/resource/om-2/"
     xmlns:geo="http://www.w3.org/2003/01/geo/wgs84_pos#"
     xmlns:owl="http://www.w3.org/2002/07/owl#"
     xmlns:rdf="http://www.w3.org/1999/02/22-rdf-syntax-ns#"
     xmlns:xml="http://www.w3.org/XML/1998/namespace"
     xmlns:xsd="http://www.w3.org/2001/XMLSchema#"
     xmlns:foaf="http://xmlns.com/foaf/0.1/"
     xmlns:rdfs="http://www.w3.org/2000/01/rdf-schema#"
     xmlns:skos="http://www.w3.org/2004/02/skos/core#"
     xmlns:sosa="http://www.w3.org/ns/sosa/"
     xmlns:vann="http://purl.org/vocab/vann/"
     xmlns:terms="http://purl.org/dc/terms/"
     xmlns:schema="http://schema.org/">
    <owl:Ontology rdf:about="http://smartcities.linkeddata.es/airQuality/ontology">
        <owl:imports rdf:resource="http://www.w3.org/ns/sosa/"/>
    </owl:Ontology>
    


    <!-- 
    ///////////////////////////////////////////////////////////////////////////////////////
    //
    // Object Properties
    //
    ///////////////////////////////////////////////////////////////////////////////////////
     -->

    


    <!-- http://schema.org/address -->

    <owl:ObjectProperty rdf:about="http://schema.org/address"/>
    


    <!-- http://schema.org/containedInPlace -->

    <owl:ObjectProperty rdf:about="http://schema.org/containedInPlace"/>
    


    <!-- http://smartcities.linkeddata.es/airQuality/ontology#fechaAlta -->

    <owl:ObjectProperty rdf:about="http://smartcities.linkeddata.es/airQuality/ontology#fechaAlta">
        <schema:domainIncludes rdf:resource="http://www.w3.org/ns/sosa/Platform"/>
        <rdfs:comment xml:lang="en">Date when the measurement station started working</rdfs:comment>
        <rdfs:comment xml:lang="es">Fecha de comienzo de funcionamiento de una estación de medición</rdfs:comment>
        <skos:definition xml:lang="en">Date when the measurement station started working</skos:definition>
        <skos:definition xml:lang="es">Fecha de comienzo de funcionamiento de una estación de medición</skos:definition>
    </owl:ObjectProperty>
    


    <!-- http://smartcities.linkeddata.es/airQuality/ontology#hasTecnica -->

    <owl:ObjectProperty rdf:about="http://smartcities.linkeddata.es/airQuality/ontology#hasTecnica">
        <schema:domainIncludes rdf:resource="http://www.w3.org/ns/sosa/ObservableProperty"/>
        <schema:rangeIncludes rdf:resource="http://smartcities.linkeddata.es/airQuality/ontology#Tecnica"/>
        <rdfs:comment xml:lang="es">Describe la técnica utilizada para la medición de cierta magnitud</rdfs:comment>
        <rdfs:comment xml:lang="en">Describes the technique utilized to measure certain magnitude</rdfs:comment>
        <skos:definition xml:lang="es">Describe la técnica utilizada para la medición de cierta magnitud</skos:definition>
        <skos:definition xml:lang="en">Describes the technique utilized to measure certain magnitude</skos:definition>
    </owl:ObjectProperty>
    


    <!-- http://smartcities.linkeddata.es/airQuality/ontology#isValid -->

    <owl:ObjectProperty rdf:about="http://smartcities.linkeddata.es/airQuality/ontology#isValid">
        <schema:domainIncludes rdf:resource="http://www.w3.org/ns/sosa/Observation"/>
        <schema:rangeIncludes rdf:resource="http://www.w3.org/2000/01/rdf-schema#Literal"/>
        <rdfs:comment xml:lang="es">Describe si una observación tiene un resultado válido (V), temporalmente válido (T), o inválido (N).</rdfs:comment>
        <rdfs:comment xml:lang="en">Describes if an observation has a valid (V), a temporally valid (T) or an invalid (N) result</rdfs:comment>
        <skos:definition xml:lang="es">Describe si una observación tiene un resultado válido (V), temporalmente válido (T), o inválido (N).</skos:definition>
        <skos:definition xml:lang="en">Describes if an observation has a valid (V), a temporally valid (T) or an invalid (N) result</skos:definition>
    </owl:ObjectProperty>
    


    <!-- http://smartcities.linkeddata.es/airQuality/ontology#tipoEstacion -->

    <owl:ObjectProperty rdf:about="http://smartcities.linkeddata.es/airQuality/ontology#tipoEstacion">
        <schema:domainIncludes rdf:resource="http://www.w3.org/ns/sosa/Platform"/>
        <rdfs:comment xml:lang="es">El tipo de una determinada estación de medida. Puede ser &apos;Trafico&apos;, &apos;Industrial&apos; o &apos;Fondo&apos;</rdfs:comment>
        <rdfs:comment xml:lang="en">The type of a measurement station. It could be &quot;Trafico&quot;, &quot;Industrial&quot; o &quot;Fondo&quot;</rdfs:comment>
        <skos:definition xml:lang="es">El tipo de una determinada estación de medida. Puede ser &apos;Trafico&apos;, &apos;Industrial&apos; o &apos;Fondo&apos;</skos:definition>
        <skos:definition xml:lang="en">The type of a measurement station. It could be &quot;Trafico&quot;, &quot;Industrial&quot; o &quot;Fondo&quot;</skos:definition>
    </owl:ObjectProperty>
    


    <!-- http://smartcities.linkeddata.es/airQuality/ontology#tipoLocalizacion -->

    <owl:ObjectProperty rdf:about="http://smartcities.linkeddata.es/airQuality/ontology#tipoLocalizacion">
        <schema:domainIncludes rdf:resource="http://www.w3.org/ns/sosa/Platform"/>
        <schema:rangeIncludes rdf:resource="http://www.w3.org/2000/01/rdf-schema#Literal"/>
        <rdfs:comment xml:lang="es">La zona donde una estación está ubicada</rdfs:comment>
        <rdfs:comment xml:lang="en">The zone where the station is located</rdfs:comment>
        <skos:definition xml:lang="es">La zona donde una estación está ubicada</skos:definition>
        <skos:definition xml:lang="en">The zone where the station is located</skos:definition>
    </owl:ObjectProperty>
    


    <!-- http://smartcities.linkeddata.es/airQuality/ontology#zonaEstacion -->

    <owl:ObjectProperty rdf:about="http://smartcities.linkeddata.es/airQuality/ontology#zonaEstacion">
        <schema:domainIncludes rdf:resource="http://www.w3.org/ns/sosa/Platform"/>
        <schema:rangeIncludes rdf:resource="http://www.w3.org/2000/01/rdf-schema#Literal"/>
        <rdfs:comment xml:lang="es">Tipo de zona donde la estación está ubicada</rdfs:comment>
        <rdfs:comment xml:lang="en">Type of zone where the station is located</rdfs:comment>
        <skos:definition xml:lang="es">Tipo de zona donde la estación está ubicada</skos:definition>
        <skos:definition xml:lang="en">Type of zone where the station is located</skos:definition>
    </owl:ObjectProperty>
    


    <!-- http://www.ontology-of-units-of-measure.org/resource/om-2/hasNumericalValue -->

    <owl:ObjectProperty rdf:about="http://www.ontology-of-units-of-measure.org/resource/om-2/hasNumericalValue"/>
    


    <!-- http://www.w3.org/2003/01/geo/wgs84_pos#alt -->

    <owl:ObjectProperty rdf:about="http://www.w3.org/2003/01/geo/wgs84_pos#alt"/>
    


    <!-- http://www.w3.org/2003/01/geo/wgs84_pos#lat -->

    <owl:ObjectProperty rdf:about="http://www.w3.org/2003/01/geo/wgs84_pos#lat"/>
    


    <!-- http://www.w3.org/2003/01/geo/wgs84_pos#long -->

    <owl:ObjectProperty rdf:about="http://www.w3.org/2003/01/geo/wgs84_pos#long"/>
    


    <!-- 
    ///////////////////////////////////////////////////////////////////////////////////////
    //
    // Classes
    //
    ///////////////////////////////////////////////////////////////////////////////////////
     -->

    


    <!-- http://schema.org/Place -->

    <owl:Class rdf:about="http://schema.org/Place"/>
    


    <!-- http://schema.org/PostalAddress -->

    <owl:Class rdf:about="http://schema.org/PostalAddress"/>
    


    <!-- http://smartcities.linkeddata.es/airQuality/ontology#Tecnica -->

    <owl:Class rdf:about="http://smartcities.linkeddata.es/airQuality/ontology#Tecnica"/>
    


    <!-- http://smartcities.linkeddata.es/airQuality/ontology#Unidad -->

    <owl:Class rdf:about="http://smartcities.linkeddata.es/airQuality/ontology#Unidad"/>
    


    <!-- http://www.ontology-of-units-of-measure.org/resource/om-2/Unit -->

    <owl:Class rdf:about="http://www.ontology-of-units-of-measure.org/resource/om-2/Unit"/>
    


    <!-- http://www.w3.org/2000/01/rdf-schema#Literal -->

    <owl:Class rdf:about="http://www.w3.org/2000/01/rdf-schema#Literal"/>
</rdf:RDF>



<!-- Generated by the OWL API (version 4.5.9.2019-02-01T07:24:44Z) https://github.com/owlcs/owlapi -->

